Reorgnized BiGrammar.v; moved some common wf_bigrammar constructors from Decode.v to BiGrammar.v.
Next: change the tactic ibr_simpl to use the hintdb style to make it extensible.

x86model/Model/BiGrammar.v
@@ -182,7 +182,7 @@ Fixpoint interp (t:type) : Type :=
 (* Notation [[ t ]] would interfere with "destruct H as [v [H2 H4]]" *)
 Notation "[| t |]" := (interp t).
 
-(** a pair of a function and its inverse *)
+(** A pair of a function and its inverse *)
 Notation funinv t1 t2 := (([|t1|] -> [|t2|]) * 
                           ([|t2|] -> option ([|t1|])))%type.
 
@@ -211,9 +211,10 @@ Inductive bigrammar : type -> Type :=
 Implicit Arguments Map [t1 t2].
 
 (** Denotation of Bi-Grammars *)
-(** I'm a little annoyed that I had to break out so many equalities, but
-    found this worked a little better for both inversion and proving. *)
-Inductive in_bigrammar : forall t, bigrammar t -> list char_p -> (interp t) -> Prop := 
+(* I'm a little annoyed that I had to break out so many equalities, but
+   found this worked a little better for both inversion and proving. *)
+Inductive in_bigrammar : 
+  forall t, bigrammar t -> list char_p -> (interp t) -> Prop := 
 | InEps : forall s v, s = nil -> v = tt -> in_bigrammar Eps s v
 | InChar : forall c s v, s = c::nil -> v = c -> in_bigrammar (Char c) s v
 | InAny : forall c s v, s = c::nil -> v = c -> in_bigrammar Any s v
@@ -291,11 +292,15 @@ Ltac in_bigrammar_inv :=
     match goal with 
       | [ H : in_bigrammar Eps _ _ |- _ ] => generalize (EpsInv H) ; clear H; intro
       | [ H : in_bigrammar Any _ _ |- _ ] => generalize (AnyInv H) ; clear H; intro
-      | [ H : in_bigrammar (Char _) _ _ |- _ ] => generalize (CharInv H) ; clear H; intro
-      | [ H : in_bigrammar (Alt _ _) _ _ |- _ ] => generalize (AltInv H) ; clear H; intro
-      | [ H : in_bigrammar (Cat _ _) _ _ |- _ ] => generalize (CatInv H) ; clear H; intro
+      | [ H : in_bigrammar (Char _) _ _ |- _ ] => 
+        generalize (CharInv H) ; clear H; intro
+      | [ H : in_bigrammar (Alt _ _) _ _ |- _ ] => 
+        generalize (AltInv H) ; clear H; intro
+      | [ H : in_bigrammar (Cat _ _) _ _ |- _ ] => 
+        generalize (CatInv H) ; clear H; intro
       | [ H : in_bigrammar (Zero _) _ _ |- _ ] => contradiction (ZeroInv H)
-      | [ H : in_bigrammar (Map _ _) _ _ |- _ ] => generalize (MapInv H) ; clear H; intro
+      | [ H : in_bigrammar (Map _ _) _ _ |- _ ] => 
+        generalize (MapInv H) ; clear H; intro
       | _ => idtac
     end.
 
@@ -367,8 +372,9 @@ Fixpoint wf_grammar t (g:bigrammar t) : Prop :=
 Notation wf_bigrammar t := {g:bigrammar t | wf_grammar g}.
 
 Create HintDb ibr_rng_db.
-Create HintDb inv_db.
-
+Require Import Bits.
+(* "Create HintDb inv_db" would not create an empty rewrite db *)
+Hint Rewrite Word.bits_of_Z_of_bits Word.Z_of_bits_of_Z : inv_db.
 
 (** convert variables of grammar types to their interpreted types *)
 Ltac simpl_grammar_ty :=
@@ -397,8 +403,76 @@ Ltac invertible_tac :=
   compute [snd fst]; intros;
   [try (printable_tac; fail) | try (parsable_tac; fail)].
 
-(********************************* Pretty Printer *************************************)
+Local Ltac localsimpl :=
+  repeat
+    match goal with
+      | [v: unit |- _ ] => destruct v
+      | [ |- context[char_dec ?x ?y] ] => destruct (char_dec x y)
+      | [_: context[char_dec ?x ?y] |- _] => destruct (char_dec x y)
+      | [H: wf_bigrammar _ |- _] => destruct H
+      | _ => unfold invertible, printable, parsable, in_bigrammar_rng in *;
+            in_bigrammar_inv; crush
+    end.
 
+(** * Lemmas about in_bigrammar_rng and other defs*)
+
+Lemma in_bigrammar_rng_eps: in_bigrammar_rng Eps ().
+Proof. unfold in_bigrammar_rng; crush. Qed.
+
+Lemma in_bigrammar_rng_alt_inl
+      t1 t2 (g1:bigrammar t1) (g2:bigrammar t2) (v:[|t1|]) :
+  in_bigrammar_rng (Alt g1 g2) (inl v) <->
+  in_bigrammar_rng g1 v. 
+Proof. localsimpl. Qed.
+
+Lemma in_bigrammar_rng_alt_inr
+      t1 t2 (g1:bigrammar t1) (g2:bigrammar t2) (v:[|t2|]) :
+  in_bigrammar_rng (Alt g1 g2) (inr v) <->
+  in_bigrammar_rng g2 v. 
+Proof. localsimpl. Qed.
+
+Lemma in_bigrammar_rng_cat
+      t1 t2 (g1:bigrammar t1) (g2:bigrammar t2) (v1:[|t1|]) (v2:[|t2|]) :
+  in_bigrammar_rng (Cat g1 g2) (v1, v2) <->
+  in_bigrammar_rng g1 v1 /\ in_bigrammar_rng g2 v2. 
+Proof. localsimpl. Qed.
+
+Lemma in_bigrammar_rng_map t1 t2 (g:bigrammar t1) (fi: funinv t1 t2) v:
+  (exists v', in_bigrammar_rng g v' /\ v = fst fi v') <->
+  in_bigrammar_rng (Map fi g) v.
+Proof. localsimpl. Qed.
+
+Lemma in_bigrammar_rng_map2 t1 t2 (g:bigrammar t1) (fi: funinv t1 t2) v:
+  in_bigrammar_rng g v ->
+  in_bigrammar_rng (Map fi g) (fst fi v).
+Proof. localsimpl. Qed.
+
+Lemma strong_inv_imp_inv t1 t2 (fi: funinv t1 t2) g : 
+  strong_invertible fi -> invertible fi g.
+Proof. unfold strong_invertible, invertible, printable, parsable. crush. Qed.
+
+Lemma compose_invertible
+      t1 t2 t3 (g:bigrammar t1) (fi1:funinv t1 t2) (fi2: funinv t2 t3):
+      invertible fi1 g -> invertible fi2 (Map fi1 g) ->
+      invertible (funinv_compose fi2 fi1) g.
+Proof. 
+  unfold invertible, printable, parsable; 
+  intros; break_hyp; simpl; unfold compose.
+  split; intros;
+  use_lemma (@in_bigrammar_rng_map2 _ _ g fi1) by crush.
+  - match goal with
+      | [H: forall x, in_bigrammar_rng (Map fi1 g) _ -> _ |- _] =>
+        guess (fst fi1 v) H; localsimpl
+    end.
+  - remember_head_in_hyp as sf.
+    destruct sf; try discriminate.
+    match goal with
+      | [H: forall V W, _ -> _ -> fst fi1 V = W |- _] => 
+        erewrite H in * by eauto; crush
+    end.
+Qed.
+
+(** * Pretty printer and its correctness lemmas *)
 Fixpoint pretty_print t (g:bigrammar t) : interp t -> option (list char_p) :=
   match g in bigrammar t' return interp t' -> option (list char_p) with
     | Eps => fun v => Some nil
@@ -441,105 +515,30 @@ Fixpoint pretty_print t (g:bigrammar t) : interp t -> option (list char_p) :=
       fun v => x <- snd fi v; pretty_print g x
   end.
 
-Local Ltac localsimpl :=
-  repeat
-    match goal with
-      | [v: unit |- _ ] => destruct v
-      | [ |- context[char_dec ?x ?y] ] => destruct (char_dec x y)
-      | [_: context[char_dec ?x ?y] |- _] => destruct (char_dec x y)
-      | [H: wf_bigrammar _ |- _] => destruct H
-      | _ => unfold invertible, printable, parsable, in_bigrammar_rng in *; 
-            in_bigrammar_inv; crush
-    end.
-
-Lemma in_bigrammar_rng_eps: in_bigrammar_rng Eps ().
-Proof. unfold in_bigrammar_rng; crush. Qed.
-
-Lemma in_bigrammar_rng_alt_inl
-      t1 t2 (g1:bigrammar t1) (g2:bigrammar t2) (v:[|t1|]) :
-  in_bigrammar_rng (Alt g1 g2) (inl v) <->
-  in_bigrammar_rng g1 v. 
-Proof. localsimpl. Qed.
-
-Lemma in_bigrammar_rng_alt_inr
-      t1 t2 (g1:bigrammar t1) (g2:bigrammar t2) (v:[|t2|]) :
-  in_bigrammar_rng (Alt g1 g2) (inr v) <->
-  in_bigrammar_rng g2 v. 
-Proof. localsimpl. Qed.
-
-Lemma in_bigrammar_rng_cat
-      t1 t2 (g1:bigrammar t1) (g2:bigrammar t2) (v1:[|t1|]) (v2:[|t2|]) :
-  in_bigrammar_rng (Cat g1 g2) (v1, v2) <->
-  in_bigrammar_rng g1 v1 /\ in_bigrammar_rng g2 v2. 
-Proof. localsimpl. Qed.
-
-Lemma in_bigrammar_rng_map t1 t2 (g:bigrammar t1) (fi: funinv t1 t2) v:
-  (exists v', in_bigrammar_rng g v' /\ v = fst fi v') <->
-  in_bigrammar_rng (Map fi g) v.
-Proof. localsimpl. Qed.
-
-Lemma in_bigrammar_rng_map2 t1 t2 (g:bigrammar t1) (fi: funinv t1 t2) v:
-  in_bigrammar_rng g v ->
-  in_bigrammar_rng (Map fi g) (fst fi v).
-Proof. localsimpl. Qed.
-
-Ltac ibr_simpl :=
-  repeat match goal with 
-           | [H: in_bigrammar_rng (Alt _ _) (inl _) |- _] =>
-             apply in_bigrammar_rng_alt_inl in H
-           | [H: in_bigrammar_rng (Alt _ _) (inr _) |- _] =>
-             apply in_bigrammar_rng_alt_inr in H
-           | [H: in_bigrammar_rng (Map _ _) _ |- _] =>
-             apply in_bigrammar_rng_map in H; 
-               destruct H as [_ [_ _]]
-           | [ |- in_bigrammar_rng (Alt _ _) (inl _)] => 
-             apply in_bigrammar_rng_alt_inl
-           | [ |- in_bigrammar_rng (Alt _ _) (inr _)] => 
-             apply in_bigrammar_rng_alt_inr
-           | [H: in_bigrammar_rng (Cat _ _) (_,_) |- _] => 
-             apply in_bigrammar_rng_cat in H; destruct H
-           | [ |- in_bigrammar_rng (Cat _ _) (_,_) ] => 
-             apply in_bigrammar_rng_cat; split
-           | [ |- in_bigrammar_rng (Map ?fi _) (fst _ _) ] =>
-             apply in_bigrammar_rng_map2
-           | [ |- in_bigrammar_rng (Map ?fi _) _ ] =>
-             apply in_bigrammar_rng_map
-           | [ |- in_bigrammar_rng Eps () ] =>
-             apply in_bigrammar_rng_eps
-           | _ => auto with ibr_rng_db
-         end.
-
-(* Ltac guess_in_all v := *)
-(*   match goal with  *)
-(*     | [H: forall x: ?T, _ |- _] => *)
-(*       match type of v with *)
-(*         | T => guess v H *)
-(*       end *)
-(*   end. *)
-
-Lemma strong_inv_imp_inv t1 t2 (fi: funinv t1 t2) g : 
-  strong_invertible fi -> invertible fi g.
-Proof. unfold strong_invertible, invertible, printable, parsable. crush. Qed.
-
-Lemma compose_invertible
-      t1 t2 t3 (g:bigrammar t1) (fi1:funinv t1 t2) (fi2: funinv t2 t3):
-      invertible fi1 g -> invertible fi2 (Map fi1 g) ->
-      invertible (funinv_compose fi2 fi1) g.
+Lemma pretty_print_corr1: forall t (g:bigrammar t) (v:interp t) s,
+  in_bigrammar g s v -> wf_grammar g -> exists s', pretty_print g v = Some s'.
 Proof. 
-  unfold invertible, printable, parsable; 
-  intros; break_hyp; simpl; unfold compose.
-  split; intros;
-  use_lemma (@in_bigrammar_rng_map2 _ _ g fi1) by crush.
-  - match goal with
-      | [H: forall x, in_bigrammar_rng (Map fi1 g) _ -> _ |- _] =>
-        guess (fst fi1 v) H; localsimpl
-    end.
-  - remember_head_in_hyp as sf.
-    destruct sf; try discriminate.
-    match goal with
-      | [H: forall V W, _ -> _ -> fst fi1 V = W |- _] => 
-        erewrite H in * by eauto; crush
-    end.
+  induction g; try (localsimpl; fail).
+
+  - (* Cat *)
+    localsimpl. crush_hyp.
+    
+  (* Case "Star". *)
+  (*   induction v. simprover; eauto. *)
+  (*   intros. *)
+  (*   in_inv. *)
+  (*   apply StarInv in H. *)
+  (*   simprover. *)
+  (*   assert (exists s1, pretty_print g x0 = Some s1); eauto. *)
+  (*   assert (exists s2, pretty_print (Star g) x2 = Some s2); eauto. *)
+  (*   simprover. *)
+  (*   eexists. *)
+  (*   simprover. *)
+  (*   eauto. rewrite H3. *)
+  (*   ??? *)
+  
+  - (* Map *)
+    localsimpl. guess x H1. crush.
 Qed.
 
 Lemma pretty_print_corr2: forall t (g:bigrammar t) (v:interp t) s,
@@ -571,29 +570,273 @@ Proof.
     guess v H2. crush.
 Qed.
 
-Lemma pretty_print_corr1: forall t (g:bigrammar t) (v:interp t) s,
-  in_bigrammar g s v -> wf_grammar g -> exists s', pretty_print g v = Some s'.
-Proof. 
-  induction g; try (localsimpl; fail).
 
-  - (* Cat *)
-    localsimpl. crush_hyp.
-    
-  (* Case "Star". *)
-  (*   induction v. simprover; eauto. *)
-  (*   intros. *)
-  (*   in_inv. *)
-  (*   apply StarInv in H. *)
-  (*   simprover. *)
-  (*   assert (exists s1, pretty_print g x0 = Some s1); eauto. *)
-  (*   assert (exists s2, pretty_print (Star g) x2 = Some s2); eauto. *)
-  (*   simprover. *)
-  (*   eexists. *)
-  (*   simprover. *)
-  (*   eauto. rewrite H3. *)
-  (*   ??? *)
-  
-  - (* Map *)
-    localsimpl. guess x H1. crush.
+(** * Constructors for wf bigrammars *)
+
+Local Ltac localcrush :=
+  repeat match goal with
+           | [H: wf_bigrammar _ |- wf_grammar _] => destruct H
+           | [ |- invertible _ _ ] => invertible_tac
+           | _ => crush
+         end.
+
+Obligation Tactic := localcrush.
+
+Program Definition empty : wf_bigrammar Unit_t := Eps.
+Program Definition never t : wf_bigrammar t := Zero t.
+
+Program Definition map t1 t2 (g:wf_bigrammar t1) (fi:funinv t1 t2)
+             (pf: invertible fi (` g)) : wf_bigrammar t2 := 
+  Map fi (` g).
+Implicit Arguments map [t1 t2].
+Notation "g @ f & fi & pf" :=(map g (f, fi) pf) (at level 75).
+
+(* could also have the test return option(a=b) instead of {a=b}+{a<>b}. *)
+Program Definition always t (teq: forall (a b:interp t), {a=b}+{a<>b})
+        (x:interp t) : wf_bigrammar t := 
+  Eps @ (fun (_:unit) => x) & (fun y => if teq x y then Some tt else None)
+      & _.
+Next Obligation. 
+  - destruct (teq x x).
+    + printable_tac.
+    + crush.
+  - destruct (teq x w); crush.
+Defined.
+
+Program Definition seq t1 t2 (p1:wf_bigrammar t1) (p2:wf_bigrammar t2) : 
+  wf_bigrammar (Pair_t t1 t2) :=
+  Cat p1 p2.
+
+Program Definition alt t1 t2 (p1:wf_bigrammar t1) (p2:wf_bigrammar t2) : 
+  wf_bigrammar (Sum_t t1 t2) :=
+  Alt p1 p2.
+
+
+(* Definition cons t (pair : interp (Pair_t t (List_t t))) : interp (List_t t) :=  *)
+(*   (fst pair)::(snd pair). *)
+
+(* doesn't seem that this is used; removed for now *)
+(* Definition seqs t (ps:list (wf_bigrammar t)) : wf_bigrammar (List_t t) :=  *)
+(*   List.fold_right (fun p1 p2 => map (seq p1 p2) (@cons t))  *)
+(*     (@always (List_t t) (@nil (interp t))) ps. *)
+
+
+(** A union operator for two grammars; it uses the pretty printer to try
+      the left branch; only if it fails, it tries the right branch.  This
+      operator should be avoided if possible for the following reasons.
+      Suppose we union n grammars, each of size m. Pretty-print each
+      grammar takes times linear to m.  Pretty print (g1+g2+...gn) would
+      take the worst case n*m time as it may try all n possibilities. *)
+Definition union t (g1 g2:wf_bigrammar t) : wf_bigrammar t.
+  intros.
+  refine ((alt g1 g2)
+            @ (fun w : interp (Sum_t t t) => match w with inl x => x | inr y => y end)
+            & (fun v : interp t => 
+                 match pretty_print (Alt (` g1) (` g2)) (inl _ v) with 
+                   | Some _ => Some (inl _ v)
+                   | None => match pretty_print (Alt (` g1)  (` g2)) (inr _ v) with 
+                               | Some _ => Some (inr _ v)
+                               | None => None
+                             end
+                 end)
+            & _); invertible_tac.
+  - destruct v.
+    + remember_destruct_head as v1; eauto.
+      remember_destruct_head as v2.
+      * localsimpl. eexists. eauto using pretty_print_corr1, pretty_print_corr2.
+      * localsimpl. generalize pretty_print_corr1; crush_hyp.
+    + localsimpl.
+      remember_destruct_head as v1; eauto 6 using pretty_print_corr2.
+      remember_destruct_head as v2; eauto 6.
+      generalize pretty_print_corr1; crush_hyp.
+  - remember_head_in_hyp as e1; destruct e1; try crush.
+    remember_head_in_hyp as e2; destruct e2; crush.
+Defined.
+
+Fixpoint unions0 t (ps:list (wf_bigrammar t)) : wf_bigrammar t := 
+  match ps with 
+    | nil => @never t
+    | p::nil => p
+    | p::rest => union p (unions0 rest)
+  end.
+
+Fixpoint half A (xs ys zs: list A) : (list A) * (list A) := 
+  match xs with 
+    | nil => (ys,zs) 
+    | h::t => half t zs (h::ys)
+  end.
+
+Fixpoint unions' n t (ps:list (wf_bigrammar t)) : wf_bigrammar t := 
+  match n, ps with 
+    | 0, _ => unions0 ps
+    | S n, nil => @never t
+    | S n, p::nil => p
+    | S n, ps => 
+      let (ps1,ps2) := half ps nil nil in 
+      let g1 := unions' n ps1 in 
+      let g2 := unions' n ps2 in 
+      union g1 g2
+  end.
+
+Definition unions t (ps:list (wf_bigrammar t)) : wf_bigrammar t := unions' 20 ps.
+
+(* notation for building bigrammars *)
+Infix "|+|" := alt (right associativity, at level 80).
+Infix "|\/|" := union (right associativity, at level 80).
+Infix "$" := seq (right associativity, at level 70).
+Notation "e %% t" := (e : interp t) (at level 80).
+
+Ltac ibr_simpl :=
+  repeat match goal with 
+           | [H: in_bigrammar_rng (` (_ |+| _)) _ |- _] =>
+             unfold proj1_sig at 1, alt at 1 in H
+           | [H: in_bigrammar_rng (` (_ $ _)) _ |- _] => 
+             unfold proj1_sig at 1, seq at 1 in H
+           | [H: in_bigrammar_rng (` (map _ _ _)) _ |- _] => 
+             unfold proj1_sig at 1, map in H
+           | [H: in_bigrammar_rng (Alt _ _) (inl _) |- _] =>
+             apply in_bigrammar_rng_alt_inl in H
+           | [H: in_bigrammar_rng (Alt _ _) (inr _) |- _] =>
+             apply in_bigrammar_rng_alt_inr in H
+           | [H: in_bigrammar_rng (Map _ _) _ |- _] =>
+             apply in_bigrammar_rng_map in H; 
+               let v := fresh "v" in let h1 := fresh "H" in
+               let h2 := fresh "H" in 
+               destruct H as [v [h1 h2]]; simpl in h2
+           | [H: in_bigrammar_rng (Cat _ _) (_,_) |- _] => 
+             apply in_bigrammar_rng_cat in H; destruct H
+           | [ |- in_bigrammar_rng (Alt _ _) (inl _)] => 
+             apply in_bigrammar_rng_alt_inl
+           | [ |- in_bigrammar_rng (Alt _ _) (inr _)] => 
+             apply in_bigrammar_rng_alt_inr
+           | [ |- in_bigrammar_rng (Cat _ _) (_,_) ] => 
+             apply in_bigrammar_rng_cat; split
+           | [ |- in_bigrammar_rng (Map ?fi _) (fst _ _) ] =>
+             apply in_bigrammar_rng_map2
+           | [ |- in_bigrammar_rng (Map ?fi _) _ ] =>
+             apply in_bigrammar_rng_map
+           | [ |- in_bigrammar_rng Eps () ] =>
+             apply in_bigrammar_rng_eps
+           | [ |- in_bigrammar_rng (` (_ |+| _)) _] =>
+             unfold proj1_sig at 1, alt at 1
+           | [ |- in_bigrammar_rng (` (_ $ _)) _ ] => 
+             unfold proj1_sig at 1, seq at 1
+           | [ |- in_bigrammar_rng (` (map _ _ _)) _ ] => 
+             unfold proj1_sig at 1, map
+           | _ => auto with ibr_rng_db
+         end.
+
+Definition pred_options t (g1 g2: wf_bigrammar t) := 
+  forall x: [|t|], ({in_bigrammar_rng (` g1) x} + {in_bigrammar_rng (` g2) x}) +
+                   {not (in_bigrammar_rng (` g1) x) /\ 
+                    not (in_bigrammar_rng (` g2) x)}.
+
+(** Three-way predicated union: the pretty printer for "g1 + g2" uses the
+    left one if x is in the range of g1, uses the right one if x is in
+    the range of g2, or it aborts when x is not in the range of either g1
+    or g2.*)
+Definition predicated_union_three_way t (g1 g2: wf_bigrammar t)
+           (pred: @pred_options t g1 g2) : wf_bigrammar t.
+  intros.
+  refine((alt g1 g2)
+           @ (fun v : interp (Sum_t t t) => match v with inl x => x | inr y => y end)
+           & (fun w : [|t|] => 
+                match (pred w) with
+                  | inleft (left _) => Some (inl w)
+                  | inleft (right _) => Some (inr w)
+                  | inright _ => None
+                end)
+           & _); invertible_tac.
+  - destruct v as [v|v]; simpl.
+    + destruct (pred v) as [[H2|H2]|H2];
+      try (eexists; localsimpl; fail).
+      ibr_simpl; crush.
+    + destruct (pred v) as [[H2|H2]|H2];
+      try (eexists; localsimpl; fail).
+      ibr_simpl; crush.
+  - destruct v; destruct (pred w) as [[H2|H2]|H2]; crush.
+Defined. 
+
+(** Predicated union: the pretty printer for "g1 + g2" uses the left one
+    if x is in the range of g1 and uses the right one if x is in the
+    range of g2; it bias towards g1 if x is in the range of both. *)
+Definition predicated_union t (g1 g2: wf_bigrammar t)
+           (pred: forall x:interp t,  {in_bigrammar_rng (` g1) x} + 
+                                      {in_bigrammar_rng (` g2) x}) :
+  wf_bigrammar t.
+  intros;
+  refine ((alt g1 g2)
+            @ (fun v : interp (Sum_t t t) => 
+                 match v with inl x => x | inr y => y end)
+            & (fun w : [|t|] => if (pred w) then Some (inl w) else Some (inr w))
+            & _); invertible_tac.
+  - destruct v as [v|v]; simpl;
+    destruct (pred v); printable_tac; ibr_simpl; crush.
+  - crush; destruct v; destruct (pred w); crush. 
+Defined.
+
+(* This version also works, but its extracted code is inefficient *)
+(* Program Definition predicated_union t (g1 g2: wf_bigrammar t) *)
+(*         (pred: forall x:interp t,  {in_bigrammar_rng g1 x} +  *)
+(*                                    {in_bigrammar_rng g2 x}) : *)
+(*   wf_bigrammar t :=  *)
+(*   @predicated_union_three_way t g1 g2 (fun w => inleft (pred w)). *)
+
+
+(* Left biased toward g1, for the special case when rng(g2) is 
+     a subset of rng(g1). *)
+Program Definition biased_union t (g1 g2: wf_bigrammar t)
+        (ss: bigrammar_rng_subset g2 g1) : wf_bigrammar t := 
+  (alt g1 g2) 
+    @ (fun v : interp (Sum_t t t) => match v with inl x => x | inr y => y end)
+    & (fun w : [|t|] => Some (inl w))
+    & _.
+Next Obligation.
+  destruct v; try crush.
+  eexists; crush.
+  ibr_simpl.
+Defined.
+
+(* The following def works for g1 and g2 that have different types; we
+     could use the above def together with a map that uses f to go from
+     t1 to t2, at the cost of some inefficiency. *)
+(* Definition bigrammar_rng_subset t1 t2 (g1: bigrammar t1) (f: interp t1 -> interp t2) *)
+(*            (g2: bigrammar t2) :=  *)
+(*   forall v1, in_bigrammar_rng g1 v1 -> in_bigrammar_rng g2 (f v1). *)
+(* Program Definition biased_union t1 t2 (g1: wf_bigrammar t1) (g2: wf_bigrammar t2) *)
+(*         (f: interp t2 -> interp t1) *)
+(*         (pfs: bigrammar_rng_subset g2 f g1) : wf_bigrammar t1 :=  *)
+(*   @Map (Sum_t t1 t2) t1 *)
+(*        (fun v : interp (Sum_t t1 t2) => match v with inl x => x | inr y => f y end, *)
+(*         fun w : interp t1 => Some (inl w)) *)
+(*        (Alt g1 g2). *)
+(* Next Obligation. *)
+(*   - localsimpl.  *)
+(*   - localsimpl. *)
+(*   - unfold invertible; split. *)
+(*     * intros. destruct v. crush. *)
+(*       unfold bigrammar_rng_subset, in_bigrammar_rng in *. *)
+(*       guess i pfs.  *)
+(*       assert (exists s, in_bigrammar (` g2) s i).  *)
+(*         crush. in_bigrammar_inv. crush. inversion H0. crush. *)
+(*       apply pfs in H0. *)
+(*       crush. *)
+(*     * crush. *)
+(* Defined. *)
+
+(** * Lemmas about wf bigrammar constructors *)
+
+Lemma in_bigrammar_rng_union t (g1 g2:wf_bigrammar t) v:
+  in_bigrammar_rng (` (g1 |\/| g2)) v <->
+  in_bigrammar_rng (` g1) v \/ in_bigrammar_rng (` g2) v.
+Proof. intros; unfold union; split; intros.
+  - ibr_simpl; destruct v0; ibr_simpl; crush.
+  - ibr_simpl. simpl.
+    destruct H.
+    + exists (inl [|t|] v). split; ibr_simpl.
+    + exists (inr [|t|] v). split; ibr_simpl.
 Qed.
+
+
+
 
